vale/code/arch/x64/Vale.X64.Decls.fst
@@ -43,8 +43,7 @@ let va_fuel_default () = 0
 
 let lemma_opr_Mem64 (id:heaplet_id) (s:va_state) (base:va_operand) (offset:int) (b:M.buffer64) (index:int) (t:taint) : Lemma
   (requires (
-    let h = Map16.sel s.vs_heap.vf_heaplets 0 in
-    id == 0 /\
+    let h = Map16.sel s.vs_heap.vf_heaplets id in
     M.mem_inv s.vs_heap /\
     OReg? base /\
     valid_src_addr h b index /\
@@ -53,12 +52,12 @@ let lemma_opr_Mem64 (id:heaplet_id) (s:va_state) (base:va_operand) (offset:int) 
     eval_operand base s + offset == M.buffer_addr b h + 8 * index
   ))
   (ensures (
-    let h = Map16.sel s.vs_heap.vf_heaplets 0 in
+    let h = Map16.sel s.vs_heap.vf_heaplets id in
     valid_operand (va_opr_code_Mem64 id base offset t) s /\
     M.load_mem64 (M.buffer_addr b h + 8 * index) (s.vs_heap.vf_heap) == M.buffer_read b index h
   ))
   =
-  Vale.X64.Memory_Sems.low_lemma_load_mem64_full b index s.vs_heap t;
+  Vale.X64.Memory_Sems.low_lemma_load_mem64_full b index s.vs_heap t id;
   let h = M.get_vale_heap s.vs_heap in
   let t = va_opr_code_Mem64 id base offset t in
   M.lemma_valid_mem64 b index h;
@@ -68,8 +67,7 @@ let lemma_opr_Mem64 (id:heaplet_id) (s:va_state) (base:va_operand) (offset:int) 
 
 let lemma_opr_Mem128 (id:heaplet_id) (s:va_state) (base:va_operand) (offset:int) (t:taint) (b:M.buffer128) (index:int) : Lemma
   (requires (
-    let h = Map16.sel s.vs_heap.vf_heaplets 0 in
-    id == 0 /\
+    let h = Map16.sel s.vs_heap.vf_heaplets id in
     M.mem_inv s.vs_heap /\
     OReg? base /\
     valid_src_addr h b index /\
@@ -78,12 +76,12 @@ let lemma_opr_Mem128 (id:heaplet_id) (s:va_state) (base:va_operand) (offset:int)
     eval_operand base s + offset == M.buffer_addr b h + 16 * index
   ))
   (ensures (
-    let h = Map16.sel s.vs_heap.vf_heaplets 0 in
+    let h = Map16.sel s.vs_heap.vf_heaplets id in
     valid_operand128 (va_opr_code_Mem128 id base offset t) s /\
     M.load_mem128 (M.buffer_addr b h + 16 * index) (M.get_vale_heap s.vs_heap) == M.buffer_read b index h
   ))
   =
-  Vale.X64.Memory_Sems.low_lemma_load_mem128_full b index s.vs_heap t;
+  Vale.X64.Memory_Sems.low_lemma_load_mem128_full b index s.vs_heap t id;
   let h = M.get_vale_heap s.vs_heap in
   let t = va_opr_code_Mem128 id base offset t in
   M.lemma_valid_mem128 b index h;
